# Sum of Arithmetic Sequence Formula

![rw-book-cover](https://static.qumath.in/static/next/_next/static/images/cuemath-dark-logo-9f8e8ee85028a3943d4cb7d90b9db2e7.svg)

## Metadata
- Author: [[Cuemath]]
- Full Title: Sum of Arithmetic Sequence Formula
- Category: #articles
- Summary: An arithmetic sequence is a list of numbers with a constant difference between terms. The sum of the first n terms can be found using two formulas: Sn = n/2 [2a + (n - 1)d] or Sn = n/2 [a1 + an]. These formulas help quickly add all terms in the sequence without adding each one individually.
- URL: https://www.cuemath.com/sum-of-arithmetic-sequence-formula/

## Full Document
The sum of arithmetic sequence with first term 'a' (or) a1 and common difference 'd' is denoted by Sn and can be calculated by one of the two formulas:

* Sn = n/2 [2a + (n - 1) d] (or)
* Sn = n/2 [a1 + an]

Before we begin to learn about the sum of the arithmetic sequence formula, let us recall what is an arithmetic sequence. An arithmetic sequence is a sequence of numbers where each successive term is a sum of its preceding term and a fixed number. This fixed number is called a common difference. So, in an arithmetic sequence, the differences between every two consecutive terms are the same. Let us learn the sum of arithmetic sequence formula with a few solved examples.

#### What Is the Sum of Arithmetic Sequence Formula?

The [sum of the arithmetic sequence](https://www.cuemath.com/algebra/Sum-of-arithmetic-sequence/) formula is used to calculate the sum of all the terms present in an arithmetic sequence. We know that an arithmetic series of finite [arithmetic sequence](https://www.cuemath.com/algebra/arithmetic-sequence/) follows the addition of the members that are of the form (a, a + d, a + 2d, …) where “a” = the first term and “d” = the common difference.

![Sum of Arithmetic Sequence Formula says s n equals n over 2 all times 2 a plus n minus 1 times d.](https://d138zd1ktt9iqe.cloudfront.net/media/seo_landing_files/sum-of-arithmetic-sequence-formula-1623748168.png)Sum of Arithmetic Sequence Formula says s n equals n over 2 all times 2 a plus n minus 1 times d.
##### Sum of Arithmetic Sequence Formula

Consider an arithmetic sequence (AP) whose first term is a and the [common difference](https://www.cuemath.com/algebra/common-difference/) is d.

**Formula 1:** The sum of the first n terms of an arithmetic sequence where [nth term](https://www.cuemath.com/algebra/nth-term-of-an-ap/) is not known is given by:

Sn = n/2 [2a + (n - 1) d]

Where

* Sn = the sum of the initial n terms of arithmetic sequence,
* a = the first term,
* d = the common difference between the terms,
* n = the total number of terms in the sequence and
* an = the last term of the sequence.

**Formula 2:** The sum of the first n terms of the arithmetic sequence where the nth term, Sn is known is given by:

Sn = n/2 [a1 + an]

Where

* Sn = the sum of the first n terms of the arithmetic sequence,
* a1 = the first term,
* d = the common difference,
* n = the total number of terms in the sequence and
* an = the nth term of the sequence.

#### Derivation of Sum of Arithmetic Series Formula

In an arithmetic sequence, every term after the first is obtained by adding a constant, referred to as the common difference (d).

* **Step 1:** The nth term of an arithmetic sequence, an = a1 + (n – 1)d, where the first term is a1, the second term is a1 + d, the third term is a1 + 2d, etc and this gives the sum of series formula  
 Sn = a1 + (a1 + d) + (a1 + 2d) + … + [a1 + (n–1)d] \_\_\_\_\_ eq(1)
* **Step 2:** We can also write it as,  
 Sn = an​​​ + (an – d) + (an– 2d) + … + [an – (n–1)d] \_\_\_\_\_ eq(2) (i.e., the nth term and successively subtracted the common difference)
* **Step 3:** Add the above two equations together, we get  
 2Sn = n (a1 + an) ⇒ Sn = n(a1 + an )/2. Thus, Sn = n/2(a1 + an). This is one of the formulas to find the sum of arithmetic sequence.
* **Step 4:** Substituting an = a1 + (n – 1)d,  
 Sn = n/2 [a1 + a1 + (n – 1)d]  
 Thus, Sn = n/2 [ 2a1 + (n – 1)d], which is another formula to find the sum of arithmetic series.

#### Examples Using Sum of Arithmetic Sequence Formula

**Example 1:** Find the sum of arithmetic sequence -4, -1, 2, 5, ... up to 10 terms.

**Solution:**

Here, a1 = -4 and n = 10.

Using the sum of arithmetic sequence formula,

**Answer:** Sum of arithmetic sequence -4, -1, 2, 5, ... up to 10 terms = 95.

**Example 2:** Find the sum of 7 terms of an arithmetic sequence whose first and last terms are 10 and 40 respectively.

**Solution:**

Here, a1 = 10 and a7 = 40.

Using the sum of arithmetic sequence formula,

**Answer:** Sum of 7 terms of the given arithmetic sequence = 175.

**Example 3:** Using the sum of arithmetic sequence formula, calculate the sum of the first 20 terms of the sequence 1, 5, 9, 13, ……

**Solution:**

Here, a1 = 1, d = 4 and n = 20.

Using the sum of arithmetic series formula,

**Answer:** Sum of arithmetic sequence 1, 5, 9, 13, …… (up to 20 terms) = 780.
